examples/sbf/ConFilter.v
@@ -1,30 +1,53 @@
 Require Import Coq.ZArith.BinInt.
+Require Import Coq.Program.Program.
 Require Import ProD3.examples.sbf.Utils.
 Import ListNotations.
 Open Scope Z_scope.
 
 Section ConFilter.
 
-Definition row := list bool.
+Definition row num_slots := { r: list bool | Zlength r = num_slots }.
 
-Definition frame := list row.
+Definition frame num_rows num_slots := { fr: list (row num_slots) | Zlength fr = num_rows }.
 
-Definition row_insert (r : row) (i : Z) : row :=
+Program Definition row_insert {num_slots} (r : row num_slots) (i : Z) : row num_slots :=
   upd_Znth i r true.
+Next Obligation.
+  rewrite Zlength_upd_Znth.
+  destruct r. easy.
+Qed.
 
-Definition frame_insert (f : frame) (is : list Z) : frame :=
-  map2 row_insert f is.
+Definition items size := { i: list Z | Zlength i = size }.
 
-Definition row_clear (r : row) (i : Z) : row :=
+Program Definition frame_insert {num_rows num_slots} (f : frame num_rows num_slots)
+  (is : items num_rows) : frame num_rows num_slots := map2 row_insert f is.
+Next Obligation.
+  rewrite Zlength_map2. destruct is, f. simpl. lia.
+Qed.
+
+Program Definition row_clear {num_slots} (r : row num_slots) (i : Z) : row num_slots:=
   upd_Znth i r false.
+Next Obligation.
+  rewrite Zlength_upd_Znth. destruct r. easy.
+Qed.
 
-Definition frame_clear (f : frame) (is : list Z) : frame :=
-  map2 row_clear f is.
+Program Definition empty_row num_slots (H: 0 < num_slots) : row num_slots :=
+  Zrepeat false num_slots.
+Next Obligation.
+  apply Zlength_Zrepeat. lia.
+Qed.
 
-Definition row_query (r : row) (i : Z) : bool :=
+Program Definition frame_clear {num_rows num_slots} (f : frame num_rows num_slots)
+  (is : items num_rows) : frame num_rows num_slots:= map2 row_clear f is.
+Next Obligation.
+  rewrite Zlength_map2. destruct is, f. simpl. lia.
+Qed.
+
+Program Definition row_query {num_slots} (r : row num_slots) (i : Z) : bool :=
   Znth i r.
 
-Definition frame_query (f : frame) (is : list Z) : bool :=
+Program Definition frame_query {num_rows num_slots} (f : frame num_rows num_slots)
+  (is : list Z) : bool :=
   fold_andb (map2 row_query f is).
 
 End ConFilter.
